Clean/Gadgets/Rotation64/Rotation64Bits.lean
@@ -110,12 +110,11 @@ theorem completeness (offset : Fin 8) : Completeness (F p) (elaborated offset) A
   intro i0 env x_var _ x h_input x_normalized
 
   -- simplify goal
-  set_option diagnostics true in
   simp only [main, circuit_norm, elaborated]
 
   -- we only have to prove the byte decomposition assumptions
   rw [Assumptions, U64.ByteVector.normalized_iff] at x_normalized
-  simp_all only [size, U64.ByteVector.getElem_eval_toLimbs, forall_const]
+  simp_all only [size, U64.ByteVector.getElem_eval_toLimbs, forall_const, ByteDecomposition.Assumptions]
 
 @[simps! (config := {isSimp := false, attrs := [`circuit_norm]})]
 def circuit (offset : Fin 8) : FormalCircuit (F p) U64 U64 := {
